silveroak-opentitan/aes/Acorn/Cipher.v
@@ -31,7 +31,7 @@ Import Pkg.Notations.
 Local Open Scope monad_scope.
 
 Section WithCava.
-  Context {signal} {semantics : Cava signal}.
+  Context {signal} {semantics : Cava signal} {seqsemantics : CavaSeq semantics}.
   Context {round_index round_constant : SignalType}.
 
   Context (sub_bytes:     signal Bit -> signal state -> cava (signal state))
@@ -94,110 +94,96 @@ Section WithCava.
       end.
   End Packing.
 
-  Definition cipher_round
-             (is_decrypt : signal Bit) (input: signal state) (key : signal key)
-    : cava (signal state) :=
-    (sub_bytes is_decrypt   >=>
-     shift_rows is_decrypt  >=>
-     mix_columns is_decrypt >=>
-     add_round_key key) input.
-
   Definition key_expand_and_round
              (is_decrypt : signal Bit)
-             (key_rcon_input : signal key * signal round_constant * signal state)
+             (key_rcon_data : signal cipher_state)
              (add_round_key_in_sel : signal (Vec Bit 2))
              (round_key_sel : signal Bit)
              (round_i : signal round_index)
-    : cava (signal key * signal round_constant * signal state) :=
-    let '(round_key, rcon, input) := key_rcon_input in
-    shift_rows_out <- (sub_bytes is_decrypt >=> shift_rows is_decrypt) input ;;
+    : cava (signal cipher_state) :=
+    let '(key_rcon, data) := unpair key_rcon_data in
+    let '(round_key, rcon) := unpair key_rcon in
+    shift_rows_out <- (sub_bytes is_decrypt >=> shift_rows is_decrypt) data ;;
     mix_columns_out <- mix_columns is_decrypt shift_rows_out ;;
 
     (* Different rounds perform different operations on the state before adding
        the round key; select the appropriate wire based on add_round_key_in_sel *)
     let add_round_key_in :=
-        mux4 (mkpair (mkpair (mkpair mix_columns_out input) shift_rows_out) mix_columns_out)
+        mux4 (mkpair (mkpair (mkpair mix_columns_out data) shift_rows_out) mix_columns_out)
              add_round_key_in_sel in
 
     (* Intermediate decryption rounds need to mix the key columns *)
     mixed_round_key <- inv_mix_columns_key round_key ;;
 
-    out <- add_round_key (pairSel round_key_sel (mkpair round_key mixed_round_key))
-                        add_round_key_in ;;
+    key_to_add <- muxPair round_key_sel (round_key, mixed_round_key) ;;
+    out <- add_round_key key_to_add add_round_key_in ;;
 
     (* Key expansion *)
     '(round_key, rcon) <- key_expand is_decrypt round_i (round_key, rcon) ;;
 
-    ret (round_key, rcon, out).
+    ret (mkpair (mkpair round_key rcon) out).
 
   Definition cipher_step
-             (num_rounds_regular round_0 : signal (round_index))
              (is_decrypt : signal Bit) (* called op_i in OpenTitan *)
-             (key_rcon_data : signal key * signal round_constant * signal state)
+             (is_first_round : signal Bit)
+             (num_rounds_regular : signal round_index)
+             (key_rcon_data : signal cipher_state)
              (round_i : signal round_index)
-    : cava (signal key * signal round_constant * signal state) :=
-    let '(round_key, rcon, input) := key_rcon_data in
-    is_first_round <- round_i ==? round_0 ;;
-    is_final_round <- round_i ==? num_rounds_regular ;;
+    : cava (signal cipher_state) :=
+    let '(key_rcon, data) := unpair key_rcon_data in
+    let '(round_key, rcon) := unpair key_rcon in
+    is_final_round <- round_i ==? num_rounds_regular;;
     (* add_round_key_in_sel :
        1 if round_i = 0, 2 if round_i = num_rounds_regular, 0 otherwise *)
     let add_round_key_in_sel := unpeel [is_first_round; is_final_round]%vector in
     is_middle_round <- nor2 (is_first_round, is_final_round) ;;
     (* round_key_sel : 1 for a decryption middle round, 0 otherwise *)
     round_key_sel <- and2 (is_middle_round, is_decrypt) ;;
-    key_expand_and_round is_decrypt (round_key, rcon, input)
+    key_expand_and_round is_decrypt key_rcon_data
                          add_round_key_in_sel round_key_sel round_i.
 
+  Definition cipher_loop
+    : signal cipher_signals -> cava (signal cipher_state) :=
+    loopDelayS
+      (fun input_and_state : signal cipher_signals
+                           * signal cipher_state =>
+         let '(input, feedback_state) := input_and_state in
+         (* extract signals from the input tuple *)
+         let '(input, idx) := unpair input in
+         let '(input, initial_state) := unpair input in
+         let '(input, round_0) := unpair input in
+         let '(is_decrypt, num_rounds_regular) := unpair input in
+
+         is_first_round <- idx ==? round_0 ;;
+         cipher_state <- muxPair is_first_round (feedback_state, initial_state) ;;
+         cipher_step is_decrypt is_first_round num_rounds_regular
+                     cipher_state idx).
+
   Definition cipher
-             (num_rounds_regular round_0 : signal (round_index))
+             (initial_rcon_selector : signal Bit -> cava (signal round_constant))
+             (num_rounds_regular round_0 : signal round_index)
              (is_decrypt : signal Bit) (* called op_i in OpenTitan *)
-             (initial_key : signal key) (initial_rcon : signal round_constant)
-             (round_indices : list (signal round_index)) (input : signal state)
+             (initial_key : signal key) (initial_state : signal state)
+             (round_i : signal round_index)
     : cava (signal state) :=
-    '(_, _, out) <- foldLM (cipher_step num_rounds_regular round_0 is_decrypt) round_indices
-                          (initial_key, initial_rcon, input) ;;
-    ret out.
-
-  Definition cipher_inner_loop
-             (input_and_state : signal cipher_signals * signal cipher_state)
-    : cava (signal cipher_state) :=
-    let '(input, feedback_state) := input_and_state in
-    let '(input, idx) := unpair input in
-    let '(input, initial_state) := unpair input in
-    let '(input, round_0) := unpair input in
-    let '(is_decrypt, num_rounds_regular) := unpair input in
-    is_first_round <- idx ==? round_0 ;;
-    cipher_state <- muxPair is_first_round (initial_state, feedback_state) ;;
-    let '(key_round, st) := unpair cipher_state in
-    let '(k, round) := unpair key_round in
-    '(key_round, st) <- cipher_step num_rounds_regular round_0 is_decrypt
-                                    (k, round, st) idx ;;
-    ret (mkpair (mkpair (fst key_round) (snd key_round)) st).
-
-  Context {seqsemantics : CavaSeq semantics}.
-  Context (initial_rcon: signal Bit -> cava (signal round_constant)).
-
-  Definition cipher_new
-             (num_rounds_regular round_0 : signal (round_index))
-             (is_decrypt : signal Bit) (* called op_i in OpenTitan *)
-             (initial_key : signal key)
-             (round_i : signal round_index) (input : signal state)
-    : cava (signal state) :=
-    initial_rcon <- initial_rcon is_decrypt ;;
-    let initial_state := mkpair (mkpair initial_key initial_rcon) input in
-    (* join all signals that are needed inside the cipher loop *)
-    let loop_input :=
+    initial_rcon <- initial_rcon_selector is_decrypt ;;
+    (* combine all the input signals *)
+    let initial_cipher_state : signal cipher_state :=
+        mkpair (mkpair initial_key initial_rcon) initial_state in
+    let loop_input : signal cipher_signals :=
         mkpair (mkpair (mkpair (mkpair is_decrypt num_rounds_regular)
-                                round_0) initial_state) round_i in
-    loop_out <- loopDelayS cipher_inner_loop loop_input ;;
-    let '(_, final_data) := unpair loop_out in
-    ret final_data.
+                               round_0) initial_cipher_state) round_i in
+    (* run the AES loop *)
+    loop_out <- cipher_loop loop_input ;;
+    (* select the AES state vector as output *)
+    ret (snd (unpair loop_out)).
 
   Context (num_rounds_regular round_0 round_1 round_final: signal (round_index)).
   Context (inc_round: signal round_index -> cava (signal round_index)).
 
   (* Comparable to OpenTitan aes_cipher_core but with simplified signalling *)
   Definition aes_cipher_core_simplified
+    (initial_rcon_selector : signal Bit -> cava (signal round_constant))
     (is_decrypt: signal Bit)
     (in_valid_i out_ready_i: signal Bit)
     (initial_key: signal key)
@@ -244,7 +230,8 @@ Section WithCava.
         round <- muxPair becoming_idle (round_0, next_round) ;;
 
         (* we only need to grab the state at the last round *)
-        st <- cipher_new round_final round_0 is_decrypt initial_key round initial_state ;;
+        st <- cipher initial_rcon_selector round_final round_0 is_decrypt
+                    initial_key initial_state round ;;
         buffered_state <- muxPair producing_output (st, last_buffered_state) ;;
 
         out_valid_o <- or2 (last_output_latch, producing_output) ;;
